src/Dmajortodflatmajor.v
@@ -1,1 +1,158 @@
-(* Translation here *)
+Require Import compcert.lib.Coqlib.
+Require Import compcert.lib.Maps.
+Require Import compcert.lib.Integers.
+
+Require Import compcert.common.AST.
+Require Import compcert.common.Values.
+Require Import compcert.common.Globalenvs.
+Require Import compcert.common.Memory.
+Require Import compcert.common.Events.
+Require Import compcert.common.Switch.
+Require Import compcert.common.Smallstep.
+Require Import compcert.common.Errors.
+Require compcert.backend.SelectLong.
+
+Require Import Dmajor.
+Require Import Dflatmajor.
+
+Require Import StructTact.StructTactics.
+Require Import StructTact.Util.
+
+Require Import EricTact.
+
+Section PRESERVATION.
+
+Variable prog: Dmajor.program.
+Let ge := Genv.globalenv prog.
+
+(* given a continuation, memory, injection, current stack size and current stack pointer *)
+(* need that: *)
+(* 1. current sp not in injection *)
+(* 2. current stack frame is freeable *)
+(* 1 and 2 hold for stack frames in continuation *)
+
+Definition stack_frame_wf (b : block) (stacksize : Z) (mi : meminj) (m : mem) : Prop :=
+   Mem.range_perm m b 0 stacksize Cur Freeable /\ forall b' delta, mi b' <> Some (b,delta).
+
+Lemma free_stack_frame :
+  forall mi m m' b sz,
+    Mem.mem_inj mi m m' ->
+    stack_frame_wf b sz mi m' ->
+    exists m0,
+      Mem.free m' b 0 sz = Some m0 /\ Mem.mem_inj mi m m0.
+Proof.
+  intros.
+  unfold stack_frame_wf in *.
+  break_and.
+  app Mem.range_perm_free Mem.range_perm.
+  destruct H0.
+  app Mem.free_right_inj Mem.mem_inj.
+  intros.
+  specialize (H1 b' delta). congruence.
+Qed.
+
+Definition total_inj (mi : meminj) (m : mem) : Prop :=
+  forall c b ofs v,
+    Mem.load c m b ofs = Some v ->
+    exists b',
+      mi b = Some (b',0).
+
+Definition env_inj (mi : meminj) (e e' : env) : Prop :=
+  forall id v,
+    e ! id = Some v ->
+    exists v',
+      e' ! id = Some v' /\ Val.inject mi v v'.
+
+(* HERE *)
+(* TODO do these next *)
+(* We need fact that all globals inject to same *)
+(* We need to remove stack pointer from Dmajor *)
+
+(* we need a fact about the injection *)
+(* that we'll never grab something not in the injection *)
+Lemma eval_expr_mem_inj :
+  forall ge e m sp exp v,
+    Dmajor.eval_expr ge e m sp exp v ->
+    forall m' mi e',
+      Mem.mem_inj mi m m' ->
+      total_inj mi m ->
+      env_inj mi e e' ->
+      exists v',
+        eval_expr ge e' m' sp exp v' /\ Val.inject mi v v'.
+Proof.
+  (* induction 1; intros; *)
+  (*   try (app H2 (e ! id)). *)
+  (* eexists; split; try econstructor; eauto. *)
+  (* eexists; split; try econstructor; eauto. *)
+  (* unfold Dmajor.eval_constant in *. *)
+
+  (* break_match_hyp; inv H; try econstructor; eauto. *)
+  
+  (*   try solve [eexists; split; econstructor; eauto]. *)
+  (* * app H2 (e ! id). *)
+  (* eexists. split. econstructor; eauto. *)
+  
+  (*   try solve [eexists; split; econstructor; eauto]. *)
+  
+  (* destruct vaddr; simpl in *; try congruence. *)
+  (* copy H1. *)
+  (* app H2 Mem.load. *)
+  
+  (* eapply Mem.load_inj in H1; eauto. *)
+  (* break_exists. break_and. *)
+  (* rewrite Zplus_0_r in H1. *)
+  
+  (* econstructor; try eapply IHeval_expr; eauto. *)
+  (* simpl.  *)
+  (* app Mem.load_inj Mem.mem_inj. *)
+  (* SearchAbout Mem.mem_inj. *)
+Admitted.
+
+Inductive match_states : Dmajor.state -> Dflatmajor.state -> Prop :=
+| match_state : forall f s k b e m m' z mi,
+    Mem.mem_inj mi m m' ->
+    stack_frame_wf b (fn_stackspace f) mi m' ->
+    match_states
+      (Dmajor.State f s k (Vptr b Int.zero) e m)
+      (Dflatmajor.State f s k (Vptr b Int.zero) e m' z)
+| match_callstate : forall f args k m m' z mi,
+    Mem.mem_inj mi m m' ->
+    match_states
+      (Dmajor.Callstate f args k m)
+      (Dflatmajor.Callstate f args k m' z)
+| match_returnstate : forall v k m m' z mi,
+    Mem.mem_inj mi m m' ->
+    match_states
+      (Dmajor.Returnstate v k m)
+      (Dflatmajor.Returnstate v k m' z).
+
+
+Lemma single_step_correct:
+  forall S1 t S2, Dmajor.step ge S1 t S2 ->
+  forall T1, match_states S1 T1 ->
+   (exists T2, plus Dflatmajor.step ge T1 t T2 /\ match_states S2 T2).
+Proof.
+  intros.
+  
+  inv H0; inv H;
+    try solve [eexists; split; try eapply plus_one; econstructor; eauto].
+
+  (* return from function *)
+  *
+    app free_stack_frame stack_frame_wf.
+    eexists. split. eapply plus_one.
+    econstructor; eauto.
+    econstructor; eauto.
+
+  (*  *)
+  * 
+    eexists. split. eapply plus_one.
+    econstructor; eauto.
+
+    
+Admitted.
+
+End PRESERVATION.
+
+
+    
